lib/Lib.Exponentiation.fsti
@@ -143,11 +143,6 @@ let get_bits_l (bBits:nat) (b:nat{b < pow2 bBits}) (l:pos) (i:nat{i < bBits / l}
   assert (l * (i + 1) <= bBits);
   b / pow2 (bBits - l * i - l) % pow2 l
 
-// fmul (pow k acc (pow2 l)) (pow k a (b / pow2 (bBits - l * i - l) % pow2 l))
-let exp_fw_f (#t:Type) (k:exp t) (a:t) (bBits:nat) (b:nat{b < pow2 bBits}) (l:pos) (i:nat{i < bBits / l}) (acc:t) : t
- =
-  let bits_l = get_bits_l bBits b l i in
-  fmul (exp_pow2 k acc l) (pow k a bits_l)
 
 let get_bits_c (bBits:nat) (b:nat{b < pow2 bBits}) (l:pos) : r:nat{r < pow2 l} =
   let c = bBits % l in
@@ -155,12 +150,27 @@ let get_bits_c (bBits:nat) (b:nat{b < pow2 bBits}) (l:pos) : r:nat{r < pow2 l} =
   Math.Lemmas.pow2_lt_compat l c;
   bits_c
 
-// fmul (pow k acc (pow2 c)) (pow k a (b % pow2 c))
-let exp_fw_rem (#t:Type) (k:exp t) (a:t) (bBits:nat) (b:nat{b < pow2 bBits}) (l:pos) (acc:t) : t
- =
-  let c = bBits % l in
+
+let fmul_acc_pow_a_bits_l (#t:Type) (k:exp t) (a:t) (bBits:nat) (b:nat{b < pow2 bBits}) (l:pos) (i:nat{i < bBits / l}) (acc:t) : t =
+  let bits_l = get_bits_l bBits b l i in
+  fmul acc (pow k a bits_l)
+
+let fmul_acc_pow_a_bits_c (#t:Type) (k:exp t) (a:t) (bBits:nat) (b:nat{b < pow2 bBits}) (l:pos) (acc:t) : t =
   let bits_c = get_bits_c bBits b l in
-  fmul (exp_pow2 k acc c) (pow k a bits_c)
+  fmul acc (pow k a bits_c)
+
+
+// fmul (pow k acc (pow2 l)) (pow k a (b / pow2 (bBits - l * i - l) % pow2 l))
+let exp_fw_f (#t:Type) (k:exp t) (a:t) (bBits:nat) (b:nat{b < pow2 bBits}) (l:pos) (i:nat{i < bBits / l}) (acc:t) : t =
+  let acc1 = exp_pow2 k acc l in
+  fmul_acc_pow_a_bits_l k a bBits b l i acc1
+
+
+// fmul (pow k acc (pow2 c)) (pow k a (b % pow2 c))
+let exp_fw_rem (#t:Type) (k:exp t) (a:t) (bBits:nat) (b:nat{b < pow2 bBits}) (l:pos) (acc:t) : t =
+  let c = bBits % l in
+  let acc1 = exp_pow2 k acc c in
+  fmul_acc_pow_a_bits_c k a bBits b l acc1
 
 
 let exp_fw (#t:Type) (k:exp t) (a:t) (bBits:nat) (b:nat{b < pow2 bBits}) (l:pos) : t =
@@ -176,24 +186,19 @@ val exp_fw_lemma: #t:Type -> k:exp t -> a:t -> bBits:nat -> b:nat{b < pow2 bBits
 let exp_double_fw_f (#t:Type) (k:exp t)
   (a1:t) (bBits:nat) (b1:nat{b1 < pow2 bBits})
   (a2:t) (b2:nat{b2 < pow2 bBits})
-  (l:pos) (i:nat{i < bBits / l}) (acc:t) : t =
-  let acc1 = exp_pow2 k acc l in
-  let bits_l1 = get_bits_l bBits b1 l i in
-  let bits_l2 = get_bits_l bBits b2 l i in
-  let acc2 = fmul acc1 (pow k a1 bits_l1) in
-  fmul acc2 (pow k a2 bits_l2)
+  (l:pos) (i:nat{i < bBits / l}) (acc:t) : t
+ =
+  let acc1 = exp_fw_f k a1 bBits b1 l i acc in
+  fmul_acc_pow_a_bits_l k a2 bBits b2 l i acc1
 
 
 let exp_double_fw_rem (#t:Type) (k:exp t)
   (a1:t) (bBits:nat) (b1:nat{b1 < pow2 bBits})
   (a2:t) (b2:nat{b2 < pow2 bBits})
-  (l:pos) (acc:t) : t =
-  let c = bBits % l in
-  let acc1 = exp_pow2 k acc c in
-  let bits_c1 = get_bits_c bBits b1 l in
-  let bits_c2 = get_bits_c bBits b2 l in
-  let acc2 = fmul acc1 (pow k a1 bits_c1) in
-  fmul acc2 (pow k a2 bits_c2)
+  (l:pos) (acc:t) : t
+ =
+  let acc1 = exp_fw_rem k a1 bBits b1 l acc in
+  fmul_acc_pow_a_bits_c k a2 bBits b2 l acc1
 
 
 let exp_double_fw (#t:Type) (k:exp t) (a1:t) (bBits:nat) (b1:nat{b1 < pow2 bBits}) (a2:t) (b2:nat{b2 < pow2 bBits}) (l:pos) : t =
